updates

Veritas.MultiSet.fst
@@ -72,3 +72,7 @@ let lemma_add_size (#a:eqtype) (s:mset a) (x:a):
 
 let lemma_add_elem (#a:eqtype) (s: seq a) (x: a):
   Lemma (seq2mset (append1 s x) == add_elem (seq2mset s) x) = admit()
+
+let index_of_mselem (#a:eqtype) (s: seq a) (x:a{contains x (seq2mset s)}): 
+  (i:seq_index s{index s i = x})
+  = admit()
